cava/Cava/Monad/CombinationalMonad.v
@@ -167,8 +167,10 @@ Definition greaterThanOrEqualBool {m n : nat}
 Definition bufBool (i : bool) : ident bool :=
   ret i.
 
-Definition loopBitBool (A B : SignalType) (f : combType A * bool -> ident (combType B * bool)) (a : combType A) : ident (combType B) :=
-  '(b, _) <- f (a, false) ;;
+Definition loopBool (A B C : SignalType)
+                    (f : combType A * combType C -> ident (combType B * combType C))
+                    (a : combType A) : ident (combType B) :=
+  '(b, _) <- f (a, @defaultCombValue C) ;;
   ret b.
 
 (******************************************************************************)
@@ -176,13 +178,11 @@ Definition loopBitBool (A B : SignalType) (f : combType A * bool -> ident (combT
 (* interpretation.                                                            *)
 (******************************************************************************)
 
- Instance Combinational : Cava combType :=
+ Instance CombinationalSemantics : Cava combType :=
   { cava := ident;
     zero := ret false;
     one := ret true;
     defaultSignal t := @defaultCombValue t;
-    delayBit i := ret i; (* Dummy definition for delayBit for now. *)
-    loopBit a b := @loopBitBool a b;
     inv := notBool;
     and2 := andBool;
     nand2 := nandBool;
@@ -209,6 +209,9 @@ Definition loopBitBool (A B : SignalType) (f : combType A * bool -> ident (combT
     greaterThanOrEqual m n := @greaterThanOrEqualBool m n;
     instantiate _ circuit := circuit;
     blackBox intf _ := ret (tupleInterfaceDefault (map port_type (circuitOutputs intf)));
+    (* Members that ought to be in a Sequential class. Dummy definitions. *)
+    delay _ i := ret i;
+    loop a b c := @loopBool a b c;
 }.
 
 (******************************************************************************)
