cava/Cava/Monad/Sequential.v
@@ -1,0 +1,263 @@
+(****************************************************************************)
+(* Copyright 2020 The Project Oak Authors                                   *)
+(*                                                                          *)
+(* Licensed under the Apache License, Version 2.0 (the "License")           *)
+(* you may not use this file except in compliance with the License.         *)
+(* You may obtain a copy of the License at                                  *)
+(*                                                                          *)
+(*     http://www.apache.org/licenses/LICENSE-2.0                           *)
+(*                                                                          *)
+(* Unless required by applicable law or agreed to in writing, software      *)
+(* distributed under the License is distributed on an "AS IS" BASIS,        *)
+(* WITHOUT WARRANTIES OR CONDITIONS OF ANY KIND, either express or implied. *)
+(* See the License for the specific language governing permissions and      *)
+(* limitations under the License.                                           *)
+(****************************************************************************)
+
+From Coq Require Import Bool.Bool.
+From Coq Require Import Strings.Ascii Strings.String.
+From Coq Require Import Lists.List.
+Import ListNotations.
+Require Import ExtLib.Structures.Monads.
+Require Export ExtLib.Data.Monads.IdentityMonad.
+Require Import ExtLib.Structures.Traversable.
+Export MonadNotation.
+
+Require Vector.
+From Coq Require Import Bool.Bvector.
+From Coq Require Import Fin.
+From Coq Require Import NArith.Ndigits.
+From Coq Require Import ZArith.ZArith.
+
+From Coq Require Import micromega.Lia.
+
+Require Import Cava.Cava.
+From Cava Require Import Kind.
+From Cava Require Import Signal.
+Require Import Cava.Monad.CavaClass.
+Require Import Cava.Monad.CombinationalMonad.
+
+(******************************************************************************)
+(* Loop combinator for feedback with delay.                                   *)
+(******************************************************************************)
+
+(*
+loopSeq' takes a combinational circuit f which has a pair of inputs which
+represent the current input of type A and current state of type C. This circuit
+returns a pair which represents the computed output of type B and next state
+value of type C. The list of input values for each clock tick are provided
+by the a parameter and the current state value is provided by the feedback
+parameter. The result of the loopSeq' is a list in the identity monad that
+represented the list of computed values at each tick.
+*)
+
+Fixpoint loopSeq' {A B C : SignalType}
+                  (f : seqType A * seqType C -> ident (seqType B * seqType C))
+                  (a : seqType A) (feedback: seqType C)
+  : ident (seqType B) :=
+  match a with
+  | [] => ret []
+  | x :: xs =>
+    '(yL, nextState) <- f ([x], feedback) ;; (* One step of f. *)
+    let y := hd defaultSignal yL in
+    ys <- loopSeq' f xs nextState ;; (* remaining steps of f *)
+    ret (y :: ys)
+  end.
+
+(*
+The loopSeq combinator takes a combinational circuit f which maps a pair
+representing the current input and current state to another pair
+representing the computed output and next state value. This function is used
+to compute the sequential behaviour of a circuit which uses f to iterate over
+the a inputs, using a default value for the initial state.
+*)
+
+Definition loopSeq {A B C : SignalType}
+                   (f : seqType A * seqType C -> ident (seqType B * seqType C))
+                   (a : seqType A)
+                   : ident (seqType B) :=
+  loopSeq' f a [defaultCombValue C].
+
+(******************************************************************************)
+(* A boolean sequential logic interpretation for the Cava class               *)
+(******************************************************************************)
+
+Definition notBoolList (i : list bool) : ident (list bool) :=
+  mapT notBool i.
+
+Definition andBoolList (i : (list bool) * (list bool)) : ident (list bool) :=
+  mapT andBool (combine (fst i) (snd i)).
+
+Definition nandBoolList (i : (list bool) * (list bool)) : ident (list bool) :=
+  mapT nandBool (combine (fst i) (snd i)).
+
+Definition orBoolList (i : (list bool) * (list bool)) : ident (list bool) :=
+  mapT orBool (combine (fst i) (snd i)).
+
+Definition norBoolList (i : (list bool) * (list bool)) : ident (list bool) :=
+  mapT norBool (combine (fst i) (snd i)).
+
+Definition xorBoolList (i : (list bool) * (list bool)) : ident (list bool) :=
+  mapT xorBool (combine (fst i) (snd i)).
+
+Definition xnorBoolList (i : (list bool) * (list bool)) : ident (list bool) :=
+  mapT xnorBool (combine (fst i) (snd i)).
+
+Definition lut1BoolList (f: bool -> bool) (i : list bool) : ident (list bool) :=
+  ret (map f i).
+
+Definition lut2BoolList (f: bool -> bool -> bool)
+                        (i : (list bool) * (list bool)) : ident (list bool) :=
+  ret (map (fun (i : bool * bool) => let (a, b) := i in f a b)
+           (combine (fst i) (snd i))).
+
+Definition lut3BoolList (f: bool -> bool -> bool -> bool)
+                        (i : (list bool) * (list bool) * (list bool)) : ident (list bool) :=
+  let '(aL, bL, cL) := i in
+  ret (map (fun (i : bool * bool * bool) => let '(a, b, c) := i in f a b c)
+           (combine (combine aL bL) cL)).
+
+Definition lut4BoolList (f: bool -> bool -> bool -> bool -> bool)
+                        (i : (list bool) * (list bool) * 
+                             (list bool) * (list bool)) : ident (list bool) :=
+  let '(aL, bL, cL, dL) := i in
+  ret (map (fun (i : bool * bool * bool * bool) =>
+            let '(a, b, c, d) := i in f a b c d)
+           (combine (combine (combine aL bL) cL) dL)).
+
+Definition lut5BoolList (f: bool -> bool -> bool -> bool -> bool -> bool)
+                        (i : (list bool) * (list bool) * (list bool) *
+                             (list bool) * (list bool)) : ident (list bool) :=
+  let '(aL, bL, cL, dL, eL) := i in
+  ret (map (fun (i : bool * bool * bool * bool * bool) =>
+            let '(a, b, c, d, e) := i in f a b c d e)
+           (combine (combine (combine (combine aL bL) cL) dL) eL)).
+
+Definition lut6BoolList (fn: bool -> bool -> bool -> bool -> bool -> bool -> bool)
+                        (i : (list bool) * (list bool) * (list bool) *
+                             (list bool) * (list bool) * (list bool)) :
+                        ident (list bool) :=
+  let '(aL, bL, cL, dL, eL, fL) := i in
+  ret (map (fun (i : bool * bool * bool * bool * bool * bool) =>
+            let '(a, b, c, d, e, f) := i in fn a b c d e f)
+           (combine (combine (combine (combine (combine aL bL) cL) dL) eL) fL)).
+
+Definition xorcyBoolList := xorBoolList.
+
+Definition muxcyBoolList (s : list bool) (ci : list bool) (di : list bool)  : ident (list bool) :=
+  let dici := combine di ci in
+  let s_dici := combine s dici in
+  ret (map (fun (i : bool * (bool * bool)) =>
+     let '(s, (ci, di)) := i in
+     match s with
+       | false => di
+       | true => ci
+     end) s_dici).
+
+Definition indexAtBoolList {t: SignalType}
+                       {sz isz: nat}
+                       (i : list (Vector.t (combType t) sz))
+                       (sel : list (Bvector isz)) : list (combType t) :=
+  map (fun '(i, sel) => indexAtBool i sel) (combine i sel).
+
+Definition indexConstBoolList {t: SignalType} {sz: nat}
+                              (i : list (Vector.t (combType t) sz))
+                              (sel : nat) : list (combType t) :=
+  map (fun i => indexConstBool i sel) i.
+
+Definition sliceBoolList {t: SignalType}
+                         {sz: nat}
+                         (startAt len : nat)
+                         (v: list (Vector.t (combType t) sz))
+                         (H: startAt + len <= sz) :
+                         list (Vector.t (combType t) len) :=
+  map (fun v => sliceBool startAt len v H) v.
+
+Definition peelVecList {t: SignalType} {s: nat}
+                       (v: list (Vector.t (combType t) s))
+                       : Vector.t (list (combType t)) s :=
+ Vector.map (fun i => map (fun j => indexConstBool j i) v) (vseq 0 s).
+
+Definition unpeelVecList' {t: SignalType} {s: nat}
+                         (v: Vector.t (list (combType t)) s)
+                         (l: nat)
+                         : list (Vector.t (combType t) s) :=
+  map (fun ni => Vector.map (fun vi => nth ni vi (defaultCombValue t)) v) (seq 0 l).
+
+Local Open Scope vector_scope.
+
+Definition unpeelVecList {t: SignalType} {s: nat}
+                         (v: Vector.t (list (combType t)) s)
+                         : list (Vector.t (combType t) s) :=
+  match s, v with
+  | O, _ => []
+  | S n, x::xs => unpeelVecList' v (length x)
+  | S _, [] => []
+  end.
+
+Local Open Scope list_scope.
+
+Definition unsignedAddBoolList {m n : nat}
+                               (av : list (Bvector m)) (bv : list (Bvector n)) :
+                               ident (list (Bvector (1 + max m n))) :=
+  mapT (fun '(a, b) => unsignedAddBool a b) (combine av bv).
+
+Definition unsignedMultBoolList {m n : nat}
+                                (av : list (Bvector m)) (bv : list (Bvector n)) :
+                                ident (list (Bvector (m + n))) :=
+  mapT (fun '(a, b) => unsignedMultBool a b) (combine av bv).
+
+Definition greaterThanOrEqualBoolList {m n : nat}
+                                      (av : list (Bvector m)) (bv : list (Bvector n)) :
+                                      ident (list bool) :=
+  mapT (fun '(a, b) => greaterThanOrEqualBool a b) (combine av bv).
+
+Definition bufBoolList (i : list bool) : ident (list bool) :=
+  ret i.
+
+(******************************************************************************)
+(* Instantiate the Cava class for a boolean sequential logic                  *)
+(* interpretation.                                                            *)
+(******************************************************************************)
+
+ Instance SequentialCombSemantics : Cava seqType :=
+  { cava := ident;
+    zero := ret [false];
+    one := ret [true];
+    defaultSignal t := @defaultSeqValue t;
+    inv := notBoolList;
+    and2 := andBoolList;
+    nand2 := nandBoolList;
+    or2 := orBoolList;
+    nor2 := norBoolList;
+    xor2 := xorBoolList;
+    xnor2 := xnorBoolList;
+    buf_gate := bufBoolList;
+    lut1 := lut1BoolList;
+    lut2 := lut2BoolList;
+    lut3 := lut3BoolList;
+    lut4 := lut4BoolList;
+    lut5 := lut5BoolList;
+    lut6 := lut6BoolList;
+    xorcy := xorcyBoolList;
+    muxcy := muxcyBoolList;
+    peel _ _ v := peelVecList v;
+    unpeel _ _ v := unpeelVecList v;
+    indexAt t sz isz := @indexAtBoolList t sz isz;
+    indexConst t sz := @indexConstBoolList t sz;
+    slice t sz := @sliceBoolList t sz;
+    unsignedAdd m n := @unsignedAddBoolList m n;
+    unsignedMult m n := @unsignedMultBoolList m n;
+    greaterThanOrEqual m n := @greaterThanOrEqualBoolList m n;
+    instantiate _ circuit := circuit;
+    blackBox intf _ := ret (tupleInterfaceDefaultS (map port_type (circuitOutputs intf)));
+    delay k i := ret (@defaultCombValue k :: i);
+   loop _ _ _ := loopSeq;
+}.
+
+(******************************************************************************)
+(* A function to run a monadic circuit description and return the boolean     *)
+(* behavioural simulation result.                                             *)
+(******************************************************************************)
+
+Definition sequential {a} (circuit : cava a) : a := unIdent circuit.
